Added PN counter + simpler proof

PN_counter/App.fst
@@ -6,30 +6,37 @@ open FStar.Ghost
 #set-options "--query_stats"
 
 // the concrete state type
-// e.g. for the increment only counter (icounter), concrete_st = nat
-type concrete_st = nat
+// e.g. for the PN counter, concrete_st = int
+type concrete_st = int
 
 //initial state
 let init_st = 0
 
 // operation type
-// (the only operation is increment, so unit is fine)
-type op_t = unit
+type op_t:eqtype = 
+  |Inc
+  |Dec
 
 // apply an operation to a state
-let do (s:concrete_st) (_:log_entry) : concrete_st = s + 1
+let do (s:concrete_st) (op:log_entry) : concrete_st = 
+  match snd op with
+  |Inc -> s + 1
+  |Dec -> s - 1
 
 ////////////////////////////////////////////////////////////////
 //// Sequential implementation //////
 
 // the concrete state 
-type concrete_st_s = nat
+type concrete_st_s = int
 
 // init state 
 let init_st_s = 0
 
 // apply an operation to a state 
-let do_s (s:concrete_st_s) (_:log_entry) : concrete_st_s = s + 1
+let do_s (s:concrete_st_s) (op:log_entry) : concrete_st_s = 
+  match snd op with
+  |Inc -> s + 1
+  |Dec -> s - 1
 
 //equivalence relation between the concrete states of sequential type and MRDT
 let eq (st_s:concrete_st_s) (st:concrete_st) = st_s = st
@@ -46,9 +53,24 @@ let do_eq (st_s:concrete_st_s) (st:concrete_st) (op:log_entry)
 
 ////////////////////////////////////////////////////////////////
 
+let rec count_inc (l:log) : Tot nat (decreases length l) =
+  match length l with
+  |0 -> 0
+  |_ -> match snd (head l) with
+       |Inc -> 1 + count_inc (tail l)
+       |_ -> count_inc (tail l)
+
+let rec count_dec (l:log) : Tot nat (decreases length l) =
+  match length l with
+  |0 -> 0
+  |_ -> match snd (head l) with
+       |Dec -> 1 + count_dec (tail l)
+       |_ -> count_dec (tail l)
+
 let rec lem_foldl (s:concrete_st) (l:log)
-  : Lemma (ensures (seq_foldl s l = s + length l) /\
-                   (length l > 0 ==> (seq_foldl s l = seq_foldl s (fst (un_snoc l)) + 1)))
+  : Lemma (ensures (seq_foldl s l = s + count_inc l - count_dec l) /\
+                   (length l > 0 /\ snd (Seq.last l) = Inc  ==> (seq_foldl s l = seq_foldl s (fst (Seq.un_snoc l)) + 1)) /\
+                   (length l > 0 /\ snd (Seq.last l) = Dec  ==> (seq_foldl s l = seq_foldl s (fst (Seq.un_snoc l)) - 1)))
           (decreases length l)
   = match length l with
     |0 -> ()
@@ -59,14 +81,13 @@ let resolve_conflict (x y:log_entry) : log =
   cons x (cons y empty)
 
 // concrete merge pre-condition
-let concrete_merge_pre lca a b : prop
-  = a >= lca /\ b >= lca
+let concrete_merge_pre lca a b : prop = true
 
 // concrete merge operation
 let concrete_merge (lca:concrete_st) (cst1:concrete_st) (cst2:concrete_st{concrete_merge_pre lca cst1 cst2}) 
   : concrete_st = cst1 + cst2 - lca
 
-#set-options "--z3rlimit 50"
+#push-options "--z3rlimit 50"
 let merge_prop (lca s1 s2:st)
   : Lemma (requires is_prefix (ops_of lca) (ops_of s1) /\ 
                     is_prefix (ops_of lca) (ops_of s2))
@@ -92,7 +113,9 @@ let merge_inv_s2_prop (lca s1 s2:st)
   lem_foldl init_st (ops_of lca); 
   lem_foldl init_st (ops_of s1);
   lem_foldl init_st (ops_of (inverse_st s2))
+#pop-options
 
+#push-options "--z3rlimit 100"
 let linearizable_s1_0 (lca s1 s2:st)
   : Lemma 
       (requires concrete_merge_pre (v_of lca) (v_of s1) (v_of s2) /\
@@ -101,9 +124,11 @@ let linearizable_s1_0 (lca s1 s2:st)
                 ops_of s1 = ops_of lca)
       (ensures concrete_merge (v_of lca) (v_of s1) (v_of s2) == 
                seq_foldl (v_of lca) (diff (ops_of s2) (ops_of lca))) =
-  lem_foldl (v_of lca) (diff (ops_of s2) (ops_of lca));
+  lem_foldl init_st (ops_of lca);
+  lem_foldl init_st (ops_of s1);
   lem_foldl init_st (ops_of s2);
-  lem_foldl init_st (ops_of lca)
+  split_prefix init_st (ops_of lca) (ops_of s2);
+  lem_foldl (v_of lca) (diff (ops_of s2) (ops_of lca))
 
 let linearizable_s2_0 (lca s1 s2:st)
   : Lemma 
@@ -113,13 +138,17 @@ let linearizable_s2_0 (lca s1 s2:st)
                 ops_of s2 = ops_of lca)
       (ensures concrete_merge (v_of lca) (v_of s1) (v_of s2) == 
                seq_foldl (v_of lca) (diff (ops_of s1) (ops_of lca))) =
-  lem_foldl (v_of lca) (diff (ops_of s1) (ops_of lca));
+  lem_foldl init_st (ops_of lca);
   lem_foldl init_st (ops_of s1);
-  lem_foldl init_st (ops_of lca)
+  lem_foldl init_st (ops_of s2);
+  split_prefix init_st (ops_of lca) (ops_of s1);
+  lem_foldl (v_of lca) (diff (ops_of s1) (ops_of lca))
 
-let lem_add (lca s1 s2:nat)
+let lem_add (lca s1 s2:int)
   : Lemma (ensures s1 - 1 + s2 - lca + 1 = s1 + s2 - lca /\
-                   s1 + (s2 - 1) - lca + 1 = s1 + s2 - lca)
+                   s1 + 1 + s2 - lca - 1 = s1 + s2 - lca /\
+                   s1 + (s2 - 1) - lca + 1 = s1 + s2 - lca /\
+                   s1 + (s2 + 1) - lca - 1 = s1 + s2 - lca)
   = ()
   
 let linearizable_s1_gt0 (lca s1 s2:st)
@@ -144,4 +173,4 @@ let linearizable_s2_gt0 (lca s1 s2:st)
                 concrete_merge_pre (v_of lca) (v_of s1) (v_of (inverse_st s2)))
       (ensures concrete_merge (v_of lca) (v_of s1) (v_of s2) ==
                do (concrete_merge (v_of lca) (v_of s1) (v_of (inverse_st s2))) (Seq.last (ops_of s2))) =
- lem_add (v_of lca) (v_of s1) (v_of s2)
+  lem_add (v_of lca) (v_of s1) (v_of s2)
